isabelle_code/Automata/implementation/Bool_Algebra.thy
@@ -1,0 +1,38 @@
+
+theory Bool_Algebra
+
+imports Main
+
+begin
+
+locale bool_algebra = 
+  fixes sem_intervals :: " 'b \<Rightarrow> 'a set"
+  fixes empty_intervals:: "'b \<Rightarrow> bool"
+  fixes noempty_intervals:: "'b \<Rightarrow> bool"
+  fixes intersect_intervals:: "'b \<Rightarrow> 'b \<Rightarrow> 'b"
+  fixes diff_intervals:: "'b \<Rightarrow> 'b \<Rightarrow> 'b"
+  fixes elem_intervals:: "'a  \<Rightarrow> 'b \<Rightarrow> bool"
+  fixes canonical_intervals:: "'b \<Rightarrow> bool"
+  assumes 
+    inj_semIs_aux: "\<And> l1 l2. canonical_intervals l1 \<and> canonical_intervals l2 
+                            \<and> sem_intervals l1 = sem_intervals l2 
+                 \<Longrightarrow> l1 = l2" and
+    empty_interval_sem: "canonical_intervals s \<longrightarrow> 
+                         empty_intervals s = (sem_intervals s = {})" and
+    noempty_intervals_sem: "canonical_intervals s \<longrightarrow> 
+                            noempty_intervals s =  (\<not> (empty_intervals s))" and
+    intersect_intervals_sem: "canonical_intervals s1 \<and> canonical_intervals s2 \<longrightarrow>
+                              sem_intervals (intersect_intervals s1 s2) = 
+                              (sem_intervals s1) \<inter> (sem_intervals s2) \<and>
+                              canonical_intervals (intersect_intervals s1 s2)" and
+    diff_intervals_sem: "canonical_intervals s1 \<and> canonical_intervals s2 \<longrightarrow>
+                              sem_intervals (diff_intervals s1 s2) = 
+                              (sem_intervals s1) - (sem_intervals s2) \<and>
+                              canonical_intervals (diff_intervals s1 s2)" and
+    elem_sem: "elem_intervals a s \<equiv>  (a \<in> sem_intervals s)"
+begin 
+
+end
+
+end
+
